WP_revisited: porting in progress

examples/WP_revisited/blocking_semantics5/blocking_semantics5_HoareLogic_many_steps_seq_1.v
@@ -40,8 +40,8 @@ Axiom mident : Type.
 Parameter mident_WhyType : WhyType mident.
 Existing Instance mident_WhyType.
 
-Axiom mident_decide : forall (m1:mident) (m2:mident), (m1 = m2) \/
-  ~ (m1 = m2).
+Axiom mident_decide :
+  forall (m1:mident) (m2:mident), (m1 = m2) \/ ~ (m1 = m2).
 
 Axiom ident : Type.
 Parameter ident_WhyType : WhyType ident.
@@ -83,158 +83,188 @@ Existing Instance stmt_WhyType.
 Axiom decide_is_skip : forall (s:stmt), (s = Sskip) \/ ~ (s = Sskip).
 
 (* Why3 assumption *)
-Definition env := (mident -> value).
+Definition env := mident -> value.
 
 (* Why3 assumption *)
 Definition stack := (list (ident* value)%type).
 
 Parameter get_stack: ident -> (list (ident* value)%type) -> value.
 
-Axiom get_stack_def : forall (i:ident) (pi:(list (ident* value)%type)),
+Axiom get_stack_def :
+  forall (i:ident) (pi:(list (ident* value)%type)),
   match pi with
   | Init.Datatypes.nil => ((get_stack i pi) = Vvoid)
-  | (Init.Datatypes.cons (x, v) r) => ((x = i) -> ((get_stack i pi) = v)) /\
-      ((~ (x = i)) -> ((get_stack i pi) = (get_stack i r)))
+  | (Init.Datatypes.cons (x, v) r) =>
+      ((x = i) -> ((get_stack i pi) = v)) /\
+      (~ (x = i) -> ((get_stack i pi) = (get_stack i r)))
   end.
 
-Axiom get_stack_eq : forall (x:ident) (v:value) (r:(list (ident*
-  value)%type)), ((get_stack x (Init.Datatypes.cons (x, v) r)) = v).
+Axiom get_stack_eq :
+  forall (x:ident) (v:value) (r:(list (ident* value)%type)),
+  ((get_stack x (Init.Datatypes.cons (x, v) r)) = v).
 
-Axiom get_stack_neq : forall (x:ident) (i:ident) (v:value) (r:(list (ident*
-  value)%type)), (~ (x = i)) -> ((get_stack i (Init.Datatypes.cons (x,
-  v) r)) = (get_stack i r)).
+Axiom get_stack_neq :
+  forall (x:ident) (i:ident) (v:value) (r:(list (ident* value)%type)),
+  ~ (x = i) ->
+  ((get_stack i (Init.Datatypes.cons (x, v) r)) = (get_stack i r)).
 
 Parameter eval_bin: value -> operator -> value -> value.
 
-Axiom eval_bin_def : forall (x:value) (op:operator) (y:value), match (x,
-  y) with
+Axiom eval_bin_def :
+  forall (x:value) (op:operator) (y:value),
+  match (x, y) with
   | ((Vint x1), (Vint y1)) =>
       match op with
       | Oplus => ((eval_bin x op y) = (Vint (x1 + y1)%Z))
       | Ominus => ((eval_bin x op y) = (Vint (x1 - y1)%Z))
       | Omult => ((eval_bin x op y) = (Vint (x1 * y1)%Z))
-      | Ole => ((x1 <= y1)%Z -> ((eval_bin x op y) = (Vbool true))) /\
-          ((~ (x1 <= y1)%Z) -> ((eval_bin x op y) = (Vbool false)))
+      | Ole =>
+          ((x1 <= y1)%Z -> ((eval_bin x op y) = (Vbool true))) /\
+          (~ (x1 <= y1)%Z -> ((eval_bin x op y) = (Vbool false)))
       end
   | (_, _) => ((eval_bin x op y) = Vvoid)
   end.
 
 (* Why3 assumption *)
-Fixpoint eval_term (sigma:(mident -> value)) (pi:(list (ident* value)%type))
+Fixpoint eval_term (sigma:mident -> value) (pi:(list (ident* value)%type))
   (t:term) {struct t}: value :=
   match t with
   | (Tvalue v) => v
-  | (Tvar id) => (get_stack id pi)
-  | (Tderef id) => (sigma id)
-  | (Tbin t1 op t2) => (eval_bin (eval_term sigma pi t1) op (eval_term sigma
-      pi t2))
+  | (Tvar id) => get_stack id pi
+  | (Tderef id) => sigma id
+  | (Tbin t1 op t2) =>
+      eval_bin (eval_term sigma pi t1) op (eval_term sigma pi t2)
   end.
 
 (* Why3 assumption *)
-Fixpoint eval_fmla (sigma:(mident -> value)) (pi:(list (ident* value)%type))
+Fixpoint eval_fmla (sigma:mident -> value) (pi:(list (ident* value)%type))
   (f:fmla) {struct f}: Prop :=
   match f with
   | (Fterm t) => ((eval_term sigma pi t) = (Vbool true))
   | (Fand f1 f2) => (eval_fmla sigma pi f1) /\ (eval_fmla sigma pi f2)
   | (Fnot f1) => ~ (eval_fmla sigma pi f1)
-  | (Fimplies f1 f2) => (eval_fmla sigma pi f1) -> (eval_fmla sigma pi f2)
-  | (Flet x t f1) => (eval_fmla sigma (Init.Datatypes.cons (x,
-      (eval_term sigma pi t)) pi) f1)
-  | (Fforall x TYint f1) => forall (n:Z), (eval_fmla sigma
-      (Init.Datatypes.cons (x, (Vint n)) pi) f1)
-  | (Fforall x TYbool f1) => forall (b:bool), (eval_fmla sigma
-      (Init.Datatypes.cons (x, (Vbool b)) pi) f1)
-  | (Fforall x TYunit f1) => (eval_fmla sigma (Init.Datatypes.cons (x,
-      Vvoid) pi) f1)
+  | (Fimplies f1 f2) => (eval_fmla sigma pi f1) -> eval_fmla sigma pi f2
+  | (Flet x t f1) =>
+      eval_fmla sigma (Init.Datatypes.cons (x, eval_term sigma pi t) pi) f1
+  | (Fforall x TYint f1) =>
+      forall (n:Z), eval_fmla sigma (Init.Datatypes.cons (x, Vint n) pi) f1
+  | (Fforall x TYbool f1) =>
+      forall (b:bool),
+      eval_fmla sigma (Init.Datatypes.cons (x, Vbool b) pi) f1
+  | (Fforall x TYunit f1) =>
+      eval_fmla sigma (Init.Datatypes.cons (x, Vvoid) pi) f1
   end.
 
 (* Why3 assumption *)
-Definition valid_fmla (p:fmla): Prop := forall (sigma:(mident -> value))
-  (pi:(list (ident* value)%type)), (eval_fmla sigma pi p).
+Definition valid_fmla (p:fmla) : Prop :=
+  forall (sigma:mident -> value) (pi:(list (ident* value)%type)),
+  eval_fmla sigma pi p.
 
 (* Why3 assumption *)
 Inductive one_step: (mident -> value) -> (list (ident* value)%type) ->
   stmt -> (mident -> value) -> (list (ident* value)%type) -> stmt -> Prop :=
-  | one_step_assign : forall (sigma:(mident -> value)) (sigma':(mident ->
-      value)) (pi:(list (ident* value)%type)) (x:mident) (t:term),
-      (sigma' = (map.Map.set sigma x (eval_term sigma pi t))) -> (one_step
-      sigma pi (Sassign x t) sigma' pi Sskip)
-  | one_step_seq_noskip : forall (sigma:(mident -> value)) (sigma':(mident ->
-      value)) (pi:(list (ident* value)%type)) (pi':(list (ident*
-      value)%type)) (s1:stmt) (s1':stmt) (s2:stmt), (one_step sigma pi s1
-      sigma' pi' s1') -> (one_step sigma pi (Sseq s1 s2) sigma' pi' (Sseq s1'
-      s2))
-  | one_step_seq_skip : forall (sigma:(mident -> value)) (pi:(list (ident*
-      value)%type)) (s:stmt), (one_step sigma pi (Sseq Sskip s) sigma pi s)
-  | one_step_if_true : forall (sigma:(mident -> value)) (pi:(list (ident*
-      value)%type)) (t:term) (s1:stmt) (s2:stmt), ((eval_term sigma pi
-      t) = (Vbool true)) -> (one_step sigma pi (Sif t s1 s2) sigma pi s1)
-  | one_step_if_false : forall (sigma:(mident -> value)) (pi:(list (ident*
-      value)%type)) (t:term) (s1:stmt) (s2:stmt), ((eval_term sigma pi
-      t) = (Vbool false)) -> (one_step sigma pi (Sif t s1 s2) sigma pi s2)
-  | one_step_assert : forall (sigma:(mident -> value)) (pi:(list (ident*
-      value)%type)) (f:fmla), (eval_fmla sigma pi f) -> (one_step sigma pi
-      (Sassert f) sigma pi Sskip)
-  | one_step_while_true : forall (sigma:(mident -> value)) (pi:(list (ident*
-      value)%type)) (cond:term) (inv:fmla) (body:stmt), ((eval_fmla sigma pi
-      inv) /\ ((eval_term sigma pi cond) = (Vbool true))) -> (one_step sigma
-      pi (Swhile cond inv body) sigma pi (Sseq body (Swhile cond inv body)))
-  | one_step_while_false : forall (sigma:(mident -> value)) (pi:(list (ident*
-      value)%type)) (cond:term) (inv:fmla) (body:stmt), ((eval_fmla sigma pi
-      inv) /\ ((eval_term sigma pi cond) = (Vbool false))) -> (one_step sigma
-      pi (Swhile cond inv body) sigma pi Sskip).
+  | one_step_assign :
+      forall (sigma:mident -> value) (sigma':mident -> value)
+        (pi:(list (ident* value)%type)) (x:mident) (t:term),
+      (sigma' = (map.Map.set sigma x (eval_term sigma pi t))) ->
+      one_step sigma pi (Sassign x t) sigma' pi Sskip
+  | one_step_seq_noskip :
+      forall (sigma:mident -> value) (sigma':mident -> value)
+        (pi:(list (ident* value)%type)) (pi':(list (ident* value)%type))
+        (s1:stmt) (s1':stmt) (s2:stmt),
+      (one_step sigma pi s1 sigma' pi' s1') ->
+      one_step sigma pi (Sseq s1 s2) sigma' pi' (Sseq s1' s2)
+  | one_step_seq_skip :
+      forall (sigma:mident -> value) (pi:(list (ident* value)%type)) (s:stmt),
+      one_step sigma pi (Sseq Sskip s) sigma pi s
+  | one_step_if_true :
+      forall (sigma:mident -> value) (pi:(list (ident* value)%type)) 
+        (t:term) (s1:stmt) (s2:stmt),
+      ((eval_term sigma pi t) = (Vbool true)) ->
+      one_step sigma pi (Sif t s1 s2) sigma pi s1
+  | one_step_if_false :
+      forall (sigma:mident -> value) (pi:(list (ident* value)%type)) 
+        (t:term) (s1:stmt) (s2:stmt),
+      ((eval_term sigma pi t) = (Vbool false)) ->
+      one_step sigma pi (Sif t s1 s2) sigma pi s2
+  | one_step_assert :
+      forall (sigma:mident -> value) (pi:(list (ident* value)%type)) (f:fmla),
+      (eval_fmla sigma pi f) -> one_step sigma pi (Sassert f) sigma pi Sskip
+  | one_step_while_true :
+      forall (sigma:mident -> value) (pi:(list (ident* value)%type))
+        (cond:term) (inv:fmla) (body:stmt),
+      ((eval_fmla sigma pi inv) /\
+       ((eval_term sigma pi cond) = (Vbool true))) ->
+      one_step sigma pi (Swhile cond inv body) sigma pi
+      (Sseq body (Swhile cond inv body))
+  | one_step_while_false :
+      forall (sigma:mident -> value) (pi:(list (ident* value)%type))
+        (cond:term) (inv:fmla) (body:stmt),
+      ((eval_fmla sigma pi inv) /\
+       ((eval_term sigma pi cond) = (Vbool false))) ->
+      one_step sigma pi (Swhile cond inv body) sigma pi Sskip.
 
 (* Why3 assumption *)
 Inductive many_steps: (mident -> value) -> (list (ident* value)%type) ->
-  stmt -> (mident -> value) -> (list (ident* value)%type) -> stmt -> Z ->
-  Prop :=
-  | many_steps_refl : forall (sigma:(mident -> value)) (pi:(list (ident*
-      value)%type)) (s:stmt), (many_steps sigma pi s sigma pi s 0%Z)
-  | many_steps_trans : forall (sigma1:(mident -> value)) (sigma2:(mident ->
-      value)) (sigma3:(mident -> value)) (pi1:(list (ident* value)%type))
-      (pi2:(list (ident* value)%type)) (pi3:(list (ident* value)%type))
-      (s1:stmt) (s2:stmt) (s3:stmt) (n:Z), (one_step sigma1 pi1 s1 sigma2 pi2
-      s2) -> ((many_steps sigma2 pi2 s2 sigma3 pi3 s3 n) -> (many_steps
-      sigma1 pi1 s1 sigma3 pi3 s3 (n + 1%Z)%Z)).
+  stmt -> (mident -> value) -> (list (ident* value)%type) -> stmt -> 
+  Z -> Prop :=
+  | many_steps_refl :
+      forall (sigma:mident -> value) (pi:(list (ident* value)%type)) (s:stmt),
+      many_steps sigma pi s sigma pi s 0%Z
+  | many_steps_trans :
+      forall (sigma1:mident -> value) (sigma2:mident -> value)
+        (sigma3:mident -> value) (pi1:(list (ident* value)%type))
+        (pi2:(list (ident* value)%type)) (pi3:(list (ident* value)%type))
+        (s1:stmt) (s2:stmt) (s3:stmt) (n:Z),
+      (one_step sigma1 pi1 s1 sigma2 pi2 s2) ->
+      (many_steps sigma2 pi2 s2 sigma3 pi3 s3 n) ->
+      many_steps sigma1 pi1 s1 sigma3 pi3 s3 (n + 1%Z)%Z.
 
-Axiom steps_non_neg : forall (sigma1:(mident -> value)) (sigma2:(mident ->
-  value)) (pi1:(list (ident* value)%type)) (pi2:(list (ident* value)%type))
-  (s1:stmt) (s2:stmt) (n:Z), (many_steps sigma1 pi1 s1 sigma2 pi2 s2 n) ->
-  (0%Z <= n)%Z.
+Axiom steps_non_neg :
+  forall (sigma1:mident -> value) (sigma2:mident -> value)
+    (pi1:(list (ident* value)%type)) (pi2:(list (ident* value)%type))
+    (s1:stmt) (s2:stmt) (n:Z),
+  (many_steps sigma1 pi1 s1 sigma2 pi2 s2 n) -> (0%Z <= n)%Z.
 
 (* Why3 assumption *)
-Definition reductible (sigma:(mident -> value)) (pi:(list (ident*
-  value)%type)) (s:stmt): Prop := exists sigma':(mident -> value),
-  exists pi':(list (ident* value)%type), exists s':stmt, (one_step sigma pi s
-  sigma' pi' s').
+Definition reductible (sigma:mident -> value) (pi:(list (ident* value)%type))
+    (s:stmt) : Prop :=
+  exists sigma':mident -> value, exists pi':(list (ident* value)%type),
+  exists s':stmt, one_step sigma pi s sigma' pi' s'.
 
-Axiom Cons_append : forall {a:Type} {a_WT:WhyType a}, forall (a1:a)
-  (l1:(list a)) (l2:(list a)),
-  ((Init.Datatypes.cons a1 (Init.Datatypes.app l1 l2)) = (Init.Datatypes.app (Init.Datatypes.cons a1 l1) l2)).
+Axiom Cons_append :
+  forall {a:Type} {a_WT:WhyType a},
+  forall (a1:a) (l1:(list a)) (l2:(list a)),
+  ((Init.Datatypes.cons a1 (Init.Datatypes.app l1 l2)) =
+   (Init.Datatypes.app (Init.Datatypes.cons a1 l1) l2)).
 
-Axiom Append_nil_l : forall {a:Type} {a_WT:WhyType a}, forall (l:(list a)),
-  ((Init.Datatypes.app Init.Datatypes.nil l) = l).
+Axiom Append_nil_l :
+  forall {a:Type} {a_WT:WhyType a},
+  forall (l:(list a)), ((Init.Datatypes.app Init.Datatypes.nil l) = l).
 
 Parameter msubst_term: term -> mident -> ident -> term.
 
-Axiom msubst_term_def : forall (t:term) (x:mident) (v:ident),
+Axiom msubst_term_def :
+  forall (t:term) (x:mident) (v:ident),
   match t with
   | ((Tvalue _)|(Tvar _)) => ((msubst_term t x v) = t)
-  | (Tderef y) => ((x = y) -> ((msubst_term t x v) = (Tvar v))) /\
-      ((~ (x = y)) -> ((msubst_term t x v) = t))
-  | (Tbin t1 op t2) => ((msubst_term t x v) = (Tbin (msubst_term t1 x v) op
-      (msubst_term t2 x v)))
+  | (Tderef y) =>
+      ((x = y) -> ((msubst_term t x v) = (Tvar v))) /\
+      (~ (x = y) -> ((msubst_term t x v) = t))
+  | (Tbin t1 op t2) =>
+      ((msubst_term t x v) =
+       (Tbin (msubst_term t1 x v) op (msubst_term t2 x v)))
   end.
 
 (* Why3 assumption *)
 Fixpoint msubst (f:fmla) (x:mident) (v:ident) {struct f}: fmla :=
   match f with
-  | (Fterm e) => (Fterm (msubst_term e x v))
-  | (Fand f1 f2) => (Fand (msubst f1 x v) (msubst f2 x v))
-  | (Fnot f1) => (Fnot (msubst f1 x v))
-  | (Fimplies f1 f2) => (Fimplies (msubst f1 x v) (msubst f2 x v))
-  | (Flet y t f1) => (Flet y (msubst_term t x v) (msubst f1 x v))
-  | (Fforall y ty f1) => (Fforall y ty (msubst f1 x v))
+  | (Fterm e) => Fterm (msubst_term e x v)
+  | (Fand f1 f2) => Fand (msubst f1 x v) (msubst f2 x v)
+  | (Fnot f1) => Fnot (msubst f1 x v)
+  | (Fimplies f1 f2) => Fimplies (msubst f1 x v) (msubst f2 x v)
+  | (Flet y t f1) => Flet y (msubst_term t x v) (msubst f1 x v)
+  | (Fforall y ty f1) => Fforall y ty (msubst f1 x v)
   end.
 
 (* Why3 assumption *)
@@ -248,68 +278,95 @@ Fixpoint fresh_in_term (id:ident) (t:term) {struct t}: Prop :=
 (* Why3 assumption *)
 Fixpoint fresh_in_fmla (id:ident) (f:fmla) {struct f}: Prop :=
   match f with
-  | (Fterm e) => (fresh_in_term id e)
-  | ((Fand f1 f2)|(Fimplies f1 f2)) => (fresh_in_fmla id f1) /\
-      (fresh_in_fmla id f2)
-  | (Fnot f1) => (fresh_in_fmla id f1)
-  | (Flet y t f1) => (~ (id = y)) /\ ((fresh_in_term id t) /\ (fresh_in_fmla
-      id f1))
-  | (Fforall y _ f1) => (~ (id = y)) /\ (fresh_in_fmla id f1)
+  | (Fterm e) => fresh_in_term id e
+  | ((Fand f1 f2)|(Fimplies f1 f2)) =>
+      (fresh_in_fmla id f1) /\ (fresh_in_fmla id f2)
+  | (Fnot f1) => fresh_in_fmla id f1
+  | (Flet y t f1) =>
+      ~ (id = y) /\ ((fresh_in_term id t) /\ (fresh_in_fmla id f1))
+  | (Fforall y _ f1) => ~ (id = y) /\ (fresh_in_fmla id f1)
   end.
 
-Axiom eval_msubst_term : forall (e:term) (sigma:(mident -> value))
-  (pi:(list (ident* value)%type)) (x:mident) (v:ident), (fresh_in_term v
-  e) -> ((eval_term sigma pi (msubst_term e x
-  v)) = (eval_term (map.Map.set sigma x (get_stack v pi)) pi e)).
+Axiom eval_msubst_term :
+  forall (e:term) (sigma:mident -> value) (pi:(list (ident* value)%type))
+    (x:mident) (v:ident),
+  (fresh_in_term v e) ->
+  ((eval_term sigma pi (msubst_term e x v)) =
+   (eval_term (map.Map.set sigma x (get_stack v pi)) pi e)).
 
-Axiom eval_msubst : forall (f:fmla) (sigma:(mident -> value))
-  (pi:(list (ident* value)%type)) (x:mident) (v:ident), (fresh_in_fmla v
-  f) -> ((eval_fmla sigma pi (msubst f x v)) <-> (eval_fmla
-  (map.Map.set sigma x (get_stack v pi)) pi f)).
+Axiom eval_msubst :
+  forall (f:fmla) (sigma:mident -> value) (pi:(list (ident* value)%type))
+    (x:mident) (v:ident),
+  (fresh_in_fmla v f) ->
+  (eval_fmla sigma pi (msubst f x v)) <->
+  (eval_fmla (map.Map.set sigma x (get_stack v pi)) pi f).
 
-Axiom eval_swap_term : forall (t:term) (sigma:(mident -> value))
-  (pi:(list (ident* value)%type)) (l:(list (ident* value)%type)) (id1:ident)
-  (id2:ident) (v1:value) (v2:value), (~ (id1 = id2)) -> ((eval_term sigma
-  (Init.Datatypes.app l (Init.Datatypes.cons (id1, v1) (Init.Datatypes.cons (
-  id2, v2) pi))) t) = (eval_term sigma
-  (Init.Datatypes.app l (Init.Datatypes.cons (id2, v2) (Init.Datatypes.cons (
-  id1, v1) pi))) t)).
+Axiom eval_swap_term :
+  forall (t:term) (sigma:mident -> value) (pi:(list (ident* value)%type))
+    (l:(list (ident* value)%type)) (id1:ident) (id2:ident) (v1:value)
+    (v2:value),
+  ~ (id1 = id2) ->
+  ((eval_term sigma
+    (Init.Datatypes.app l
+     (Init.Datatypes.cons (id1, v1) (Init.Datatypes.cons (id2, v2) pi)))
+    t)
+   =
+   (eval_term sigma
+    (Init.Datatypes.app l
+     (Init.Datatypes.cons (id2, v2) (Init.Datatypes.cons (id1, v1) pi)))
+    t)).
 
-Axiom eval_swap_gen : forall (f:fmla) (sigma:(mident -> value))
-  (pi:(list (ident* value)%type)) (l:(list (ident* value)%type)) (id1:ident)
-  (id2:ident) (v1:value) (v2:value), (~ (id1 = id2)) -> ((eval_fmla sigma
-  (Init.Datatypes.app l (Init.Datatypes.cons (id1, v1) (Init.Datatypes.cons (
-  id2, v2) pi))) f) <-> (eval_fmla sigma
-  (Init.Datatypes.app l (Init.Datatypes.cons (id2, v2) (Init.Datatypes.cons (
-  id1, v1) pi))) f)).
+Axiom eval_swap_gen :
+  forall (f:fmla) (sigma:mident -> value) (pi:(list (ident* value)%type))
+    (l:(list (ident* value)%type)) (id1:ident) (id2:ident) (v1:value)
+    (v2:value),
+  ~ (id1 = id2) ->
+  (eval_fmla sigma
+   (Init.Datatypes.app l
+    (Init.Datatypes.cons (id1, v1) (Init.Datatypes.cons (id2, v2) pi)))
+   f) <->
+  (eval_fmla sigma
+   (Init.Datatypes.app l
+    (Init.Datatypes.cons (id2, v2) (Init.Datatypes.cons (id1, v1) pi)))
+   f).
 
-Axiom eval_swap : forall (f:fmla) (sigma:(mident -> value)) (pi:(list (ident*
-  value)%type)) (id1:ident) (id2:ident) (v1:value) (v2:value),
-  (~ (id1 = id2)) -> ((eval_fmla sigma (Init.Datatypes.cons (id1,
-  v1) (Init.Datatypes.cons (id2, v2) pi)) f) <-> (eval_fmla sigma
-  (Init.Datatypes.cons (id2, v2) (Init.Datatypes.cons (id1, v1) pi)) f)).
+Axiom eval_swap :
+  forall (f:fmla) (sigma:mident -> value) (pi:(list (ident* value)%type))
+    (id1:ident) (id2:ident) (v1:value) (v2:value),
+  ~ (id1 = id2) ->
+  (eval_fmla sigma
+   (Init.Datatypes.cons (id1, v1) (Init.Datatypes.cons (id2, v2) pi)) f) <->
+  (eval_fmla sigma
+   (Init.Datatypes.cons (id2, v2) (Init.Datatypes.cons (id1, v1) pi)) f).
 
-Axiom eval_term_change_free : forall (t:term) (sigma:(mident -> value))
-  (pi:(list (ident* value)%type)) (id:ident) (v:value), (fresh_in_term id
-  t) -> ((eval_term sigma (Init.Datatypes.cons (id, v) pi)
-  t) = (eval_term sigma pi t)).
+Axiom eval_term_change_free :
+  forall (t:term) (sigma:mident -> value) (pi:(list (ident* value)%type))
+    (id:ident) (v:value),
+  (fresh_in_term id t) ->
+  ((eval_term sigma (Init.Datatypes.cons (id, v) pi) t) =
+   (eval_term sigma pi t)).
 
-Axiom eval_change_free : forall (f:fmla) (sigma:(mident -> value))
-  (pi:(list (ident* value)%type)) (id:ident) (v:value), (fresh_in_fmla id
-  f) -> ((eval_fmla sigma (Init.Datatypes.cons (id, v) pi) f) <-> (eval_fmla
-  sigma pi f)).
+Axiom eval_change_free :
+  forall (f:fmla) (sigma:mident -> value) (pi:(list (ident* value)%type))
+    (id:ident) (v:value),
+  (fresh_in_fmla id f) ->
+  (eval_fmla sigma (Init.Datatypes.cons (id, v) pi) f) <->
+  (eval_fmla sigma pi f).
 
 Require Import Why3.
 Ltac ae := why3 "Alt-Ergo,1.30," timelimit 3; admit.
 
 (* Why3 goal *)
-Theorem many_steps_seq : forall (sigma1:(mident -> value)) (sigma3:(mident ->
-  value)) (pi1:(list (ident* value)%type)) (pi3:(list (ident* value)%type))
-  (s1:stmt) (s2:stmt) (n:Z), (many_steps sigma1 pi1 (Sseq s1 s2) sigma3 pi3
-  Sskip n) -> exists sigma2:(mident -> value), exists pi2:(list (ident*
-  value)%type), exists n1:Z, exists n2:Z, (many_steps sigma1 pi1 s1 sigma2
-  pi2 Sskip n1) /\ ((many_steps sigma2 pi2 s2 sigma3 pi3 Sskip n2) /\
-  (n = ((1%Z + n1)%Z + n2)%Z)).
+Theorem many_steps_seq :
+  forall (sigma1:mident -> value) (sigma3:mident -> value)
+    (pi1:(list (ident* value)%type)) (pi3:(list (ident* value)%type))
+    (s1:stmt) (s2:stmt) (n:Z),
+  (many_steps sigma1 pi1 (Sseq s1 s2) sigma3 pi3 Sskip n) ->
+  exists sigma2:mident -> value, exists pi2:(list (ident* value)%type),
+  exists n1:Z, exists n2:Z,
+  (many_steps sigma1 pi1 s1 sigma2 pi2 Sskip n1) /\
+  ((many_steps sigma2 pi2 s2 sigma3 pi3 Sskip n2) /\
+   (n = ((1%Z + n1)%Z + n2)%Z)).
 (* Why3 intros sigma1 sigma3 pi1 pi3 s1 s2 n h1. *)
 intros sigma1 sigma3 pi1 pi3 s1 s2 n Hred.
 generalize Hred.
